add first attempt at defining Lemma 4; The goal may need some work. Specifically, currently unclear how to link a Cluster Cache Request's encapsulated requests to e_gcache downgrades to other global cache?

CompositionalProtocolProof/CompositionalProof/Lemma4ClusterRequest.lean
@@ -6,7 +6,40 @@ import CompositionalProtocolProof.CompositionalProof.Lemma5GlobalRequest
 
 variable (n : Nat)
 
+def Behaviour.dirEventCorrespondingToCacheEvent (b : Behaviour n) (init : InitialSystemState n) (e_cdir e : Event n) : Prop :=
+  b.cacheEncapsulatesCorrespondingDirEvent n (init.stateAt n e) true e_cdir e ∨
+  b.cacheEncapsulatesCorrespondingDirEvent n (init.stateAt n e) false e_cdir e
+
+def Behaviour.dirEventNotCorrespondingToCacheEvent (b : Behaviour n) (init : InitialSystemState n) (e_cdir e : Event n) : Prop :=
+  ¬ b.dirEventCorrespondingToCacheEvent n init e_cdir e
+
+structure Behaviour.clusterDirFinishBeforeUnrelated (b : Behaviour n) (init : InitialSystemState n) (e_cdir e : Event n) : Prop where
+  dirFinishBefore : e_cdir.finishesBefore n e
+  unrelated : b.dirEventNotCorrespondingToCacheEvent n init e_cdir e
+
+structure Behaviour.globalCacheFinishBeforeUnrelated (b : Behaviour n) (init : InitialSystemState n) (e_gcache e : Event n) : Prop where
+  gCacheFinishBefore : e_gcache.finishesBefore n e
+  unrelated : ∃ e_dir ∈ b, b.dirEventNotCorrespondingToCacheEvent n init e_dir e ∧ e_dir.Encapsulates n e_gcache
+
+structure Behaviour.encapCorrespondingClusterDir (b : Behaviour n) (init : InitialSystemState n) (e_cdir e : Event n) : Prop where
+  dirFinishBefore : e_cdir.Encapsulates n e
+  unrelated : b.dirEventCorrespondingToCacheEvent n init e_cdir e
+
+structure Behaviour.globalCacheFinishBefore (b : Behaviour n) (init : InitialSystemState n) (e_gcache e : Event n) : Prop where
+  gCacheFinishBefore : e_gcache.finishesBefore n e
+  unrelated : ∃ e_dir ∈ b, b.encapCorrespondingClusterDir n init e_dir e ∧ e_dir.Encapsulates n e_gcache
+
 /-- Lemma 4 : A Cluster Request Event leaves a protocol in Compound SWMR. -/
-lemma Behaviour.cluster_request_enforces_swmr (b : Behaviour n)
-  : ∀ e ∈ b, True := by
+lemma Behaviour.cluster_request_enforces_compound_swmr
+  (b : Behaviour n) (init : InitialSystemState n)
+  (cmp : CompoundProtocol n)
+  -- (hcmp_swmr : CompoundSWMR.wrapper n)
+  -- Initial or Current state just before Event `e` in Compound SWMR
+  (e : Event n) (he_in_b : e ∈ b)
+  (hpred_cdir_cmp_swmr : ∀ e_cdir ∈ b, e_cdir.isClusterDir → b.clusterDirFinishBeforeUnrelated n init e_cdir e → CompoundSWMR.stateAfterClusterDirEventLeGlobalCache n b init e_cdir)
+  (hpred_gcache_cmp_swmr : ∀ e_gcache ∈ b, e_gcache.isGlobalCache → b.globalCacheFinishBeforeUnrelated n init e_gcache e → CompoundSWMR.stateAfterClusterDirEventLeGlobalCache' n b init e_gcache)
+  : ∀ e_cdir ∈ b, e_cdir.isClusterDir → b.encapCorrespondingClusterDir n init e_cdir e → CompoundSWMR.stateAfterClusterDirEventLeGlobalCache n b init e_cdir
+  ∧
+  ∀ e_gcache ∈ b, e_gcache.isGlobalCache → b.globalCacheFinishBefore n init e_cdir e → CompoundSWMR.stateAfterClusterDirEventLeGlobalCache n b init e_cdir
+  := by
   sorry
